\documentclass[]{article}

\usepackage{graphicx}
\usepackage{longtable}
\usepackage{hyperref}
\usepackage{color}
\usepackage{soul}
\usepackage{amsmath}
\usepackage{amssymb}
\usepackage{enumitem}


\DeclareRobustCommand{\hlcyan}[1]{{\sethlcolor{cyan}\hl{#1}}}
\DeclareRobustCommand{\hlgreen}[1]{{\sethlcolor{green}\hl{#1}}}
\DeclareRobustCommand{\hlred}[1]{{\sethlcolor{red}\hl{#1}}}
\DeclareRobustCommand{\hlyellow}[1]{{\sethlcolor{yellow}\hl{#1}}}
\DeclareRobustCommand{\hlorange}[1]{{\sethlcolor{orange}\hl{#1}}}


%opening
\title{Session 11}
\author{Fakhir}

\begin{document}

\maketitle

\section*{Solutions}

\begin{enumerate}[label=(\alph*)]
	\item
	\begin{eqnarray}
	\frac{d}{dx} \left( \frac{x^{3}}{x+1} \right) & = & \frac{u'v-uv'}{v^{2}} \\
		& = & \frac{3x^{2}(x+1)-x^{3}(1)}{(x+1)^{2}} \\
		& = & \frac{x^{2}(2x+3)}{(x+1)^2}
	\end{eqnarray}
	
	\item 
	\begin{eqnarray}
	\frac{d}{dx} \left( x^{3}.(x+1)^{-1} \right) & = & u'v + uv' \\
		& = & 3x^{2}(x+1)^{-1} + x^{3}.(-1)(x+1)^{-2} \\
		& = & \frac{3x^{2}}{(x+1)} - \frac{x^{3}}{(x+1)^{2}} \\
		& = & \frac{3x^{2}(x+1)-x^{3}(1)}{(x+1)^{2}} \\
		& = & \frac{x^{2}(2x+3)}{(x+1)^2}
	\end{eqnarray}
	
	\item 
		\begin{eqnarray}
	\frac{d}{dx} u(x)(v(x))^{-1} & = & u'(x)(v(x))^{-1} + u(x).(-1)(v(x))^{-2}.v'(x) \\		
		& = & \frac{u'(x)}{v(x)} - \frac{u(x)v'(x)}{(v(x))^2} \\
		& = & \frac{u'(x)v(x) - u(x)v'(x)}{(v(x))^{2}}
	\end{eqnarray}
	
\end{enumerate}

\end{document}
